theories/theories/reactive/utp_reactive_lemmas.thy
@@ -170,6 +170,10 @@ lemma tr_leq_trans:
   "`($tr \<le> $tr\<acute>) ; ($tr \<le> $tr\<acute>)` = `($tr \<le> $tr\<acute>)`"
   sorry
 
+lemma tr_eq_is_R1:
+  "`($tr\<acute>= $tr) \<and> ($tr \<le> $tr\<acute>)` = `$tr\<acute> = $tr` "
+  sorry
+
 lemma tr_prefix_as_nil:
   "`($tr\<acute> - $tr) = \<langle>\<rangle> \<and> ($tr \<le> $tr\<acute>)` = `$tr\<acute> = $tr`"
   apply (subst prefix_eq_nil[of "tr\<acute>" "tr"])
